move address lemmas to properties

spec/Address.ec
@@ -9,15 +9,6 @@ require import Array8.
 
 require import Notation Parameters.
 
-(* TODO: Generalize to any word size *)
-lemma word_int (i : int) :
-    0 <= i < W32.modulus => W32.to_uint (W32.of_int i) = i.
-proof.
-move => pre.
-rewrite /of_int /to_uint.
-smt. (* FIXME: does not terminate if I use smt() instead of smt *)
-qed.
-
 (************************************** EXTRACTION ********************************************************************)
 (* FIXME: REMOVE THIS FROM HERE *)
 
@@ -207,70 +198,30 @@ pred set_layer_addr_pre (layer : int) = 0 <= layer.
 op set_layer_addr (address : adrs, layer : int) : adrs = 
     address.[0 <- W32.of_int layer].
 
-lemma set_layer_addr_op_impl (addr : adrs, layer: int): 
-    set_layer_addr_pre layer => 
-        hoare[M.__set_layer_addr : 
-            arg = (addr, W32.of_int layer) ==> res = set_layer_addr addr layer].
-proof. move => pre_cond. proc. auto. qed.
-
 pred set_tree_addr_pre (tree_address : int) = 0 <= tree_address.
 op set_tree_addr (address : adrs, tree_address : int) : adrs = 
-(* 
-FIXME: Should use >> instead of SHR_64.`6 but I cant prove it
-let t = (W64.of_int tree_address `>>` W8.of_int 32) in
-*)
     let t : W32.t = truncateu32 ((SHR_64 (W64.of_int tree_address) (W8.of_int 32)).`6) in
        address.[1 <- t].[2 <- (truncateu32 (W64.of_int tree_address))].
-
-lemma set_tree_addr_op_impl (address : adrs, tree_address : int):
-    set_tree_addr_pre tree_address => 
-        hoare[M.__set_tree_addr : 
-            arg = (address, W64.of_int tree_address) ==> res = set_tree_addr address tree_address].
-
-proof. move => pre_cond. proc. auto. qed.
 
 pred set_type_pre (_type : int) = 0 <= _type <= 2.
 op set_type (address : adrs, _type : int) : adrs = 
     address.[3 <- W32.of_int _type].
-lemma set_type_op_impl (address : adrs, _type : int):
-    set_type_pre _type =>
-        hoare[M.__set_type :
-            arg = (address, W32.of_int _type) ==> res = set_type address _type].
-proof. move => pre_cond. proc. auto. qed.
-
 
 (* TODO: Add Precondition *)
 op set_ots_addr (address : adrs, ots_addr : int) : adrs = 
     address.[4 <- W32.of_int ots_addr].
-lemma set_ots_addr_op_impl (address : adrs, ots_addr : int):
-    hoare[M.__set_ots_addr :
-        arg = (address, W32.of_int ots_addr) ==> res = set_ots_addr address ots_addr].
-proof. proc. auto. qed.
-
 
 (* TODO: Add Precondition *)
 op set_chain_addr (address : adrs, chain_addr : int) : adrs = 
     address.[5 <- W32.of_int chain_addr].
-lemma set_chain_addr_op_impl (address : adrs, chain_addr : int):
-    hoare[M.__set_chain_addr :
-        arg = (address, W32.of_int chain_addr) ==> res = set_chain_addr address chain_addr].
-proof. proc. auto. qed.
 
 (* TODO: Add Precondition *)
 op set_hash_addr (address : adrs, hash_addr : int) : adrs = 
     address.[6 <- W32.of_int hash_addr].
-lemma set_hash_addr_op_impl (address : adrs, hash_addr : int):
-    hoare[M.__set_hash_addr :
-        arg = (address, W32.of_int hash_addr) ==> res = set_hash_addr address hash_addr].
-proof. proc. auto. qed.
 
 (* TODO: Add Precondition *)
 op set_ltree_addr (address : adrs, ltree_addr : int) : adrs = 
     address.[4 <- W32.of_int ltree_addr].
-lemma set_ltree_addr_op_impl (address : adrs, ltree_addr : int):
-    hoare[M.__set_ltree_addr :
-        arg = (address, W32.of_int ltree_addr) ==> res = set_ltree_addr address ltree_addr].
-proof. proc. auto. qed.
 
 pred tree_height_pre (tree_height : int) = 0 <= tree_height <= XMSS_TREE_HEIGHT. 
 op set_tree_height (address : adrs, tree_height : int) : adrs = 
@@ -278,56 +229,12 @@ op set_tree_height (address : adrs, tree_height : int) : adrs =
 op get_tree_height (address : adrs) : int =
   W32.to_uint (address.[5]).
 
-lemma set_tree_height_op_impl (address : adrs, tree_height : int):
-    tree_height_pre tree_height =>
-        hoare[M.__set_tree_height :
-            arg = (address, W32.of_int tree_height) ==> res = set_tree_height address tree_height].
-proof. move => pre_cond. proc. auto. qed.
-
-lemma get_set_tree_height (address : adrs, tree_height : int) :
-    tree_height_pre tree_height => 
-    get_tree_height (set_tree_height address tree_height) = tree_height.
-proof.
-rewrite /get_tree_height /set_tree_height.
-progress.
-apply word_int.
-smt().
-qed.
-
 (* TODO: Add Precondition *)
 op set_tree_index (address : adrs, tree_index : int) : adrs = 
     address.[6 <- W32.of_int tree_index].
 
 op get_tree_index (address : adrs) : int = to_uint (address.[6]).
 
-lemma set_tree_index_op_impl (address : adrs, tree_index) : 
-    hoare[M.__set_tree_index :
-        arg = (address, W32.of_int tree_index) ==> res = set_tree_index address tree_index].
-proof. proc. auto. qed.
-
-lemma get_set_tree_index (address : adrs, tree_index : int) :
-  0 <= tree_index < W32.modulus => (* i.e. tree_index fits in a u32 *)
-  get_tree_index (set_tree_index address tree_index) = tree_index.  
-proof.
-rewrite /get_tree_index /set_tree_index.
-progress.
-apply word_int.
- smt().
-qed.
-
-
 op set_key_and_mask (address : adrs, key_and_mask : int) : adrs = 
     address.[7 <- W32.of_int key_and_mask].
-lemma set_key_and_mask_op_impl (address : adrs, key_and_mask : int):
-    hoare[M.__set_key_and_mask :
-        arg = (address, W32.of_int key_and_mask) ==> res = set_key_and_mask address key_and_mask].
-proof. proc. auto. qed.
 
-op zero_addr : adrs = Array8.init (fun _ => W32.zero). 
-lemma zero_addr_op_impl (address : adrs) :
-    hoare[M._zero_address : true ==> res = zero_addr].
-proof.
-proc.
-while (0 <= i <= 8 /\ 
-      (forall (k : int), 0 <= k < i => (addr.[k] = W32.zero))); auto => /> ; smt(get_setE tP initiE).
-qed.
