spec/Properties.ec
@@ -8,8 +8,106 @@ from Jasmin require import JModel.
 
 require import Notation Address Primitives Wots.
 
+require import Array8.
+
 import DList.
 import NBytes.
+
+(**********************************************************************************************************************)
+
+(* TODO: Generalize to any word size *)
+lemma word_int (i : int) :
+    0 <= i < W32.modulus => W32.to_uint (W32.of_int i) = i.
+proof.
+move => pre.
+rewrite /of_int /to_uint.
+smt. (* FIXME: does not terminate if I use smt() instead of smt *)
+qed.
+
+(********************************** ADDRESS ***********************************)
+
+lemma set_layer_addr_op_impl (addr : adrs, layer: int): 
+    set_layer_addr_pre layer => 
+        hoare[M.__set_layer_addr : 
+            arg = (addr, W32.of_int layer) ==> res = set_layer_addr addr layer].
+proof. move => pre_cond. proc. auto. qed.
+
+lemma set_tree_addr_op_impl (address : adrs, tree_address : int):
+    set_tree_addr_pre tree_address => 
+        hoare[M.__set_tree_addr : 
+            arg = (address, W64.of_int tree_address) ==> res = set_tree_addr address tree_address].
+proof. move => pre_cond. proc. auto. qed.
+
+lemma set_type_op_impl (address : adrs, _type : int):
+    set_type_pre _type =>
+        hoare[M.__set_type :
+            arg = (address, W32.of_int _type) ==> res = set_type address _type].
+proof. move => pre_cond. proc. auto. qed.
+
+lemma set_ots_addr_op_impl (address : adrs, ots_addr : int):
+    hoare[M.__set_ots_addr :
+        arg = (address, W32.of_int ots_addr) ==> res = set_ots_addr address ots_addr].
+proof. proc. auto. qed.
+
+lemma set_chain_addr_op_impl (address : adrs, chain_addr : int):
+    hoare[M.__set_chain_addr :
+        arg = (address, W32.of_int chain_addr) ==> res = set_chain_addr address chain_addr].
+proof. proc. auto. qed.
+
+lemma set_hash_addr_op_impl (address : adrs, hash_addr : int):
+    hoare[M.__set_hash_addr :
+        arg = (address, W32.of_int hash_addr) ==> res = set_hash_addr address hash_addr].
+proof. proc. auto. qed.
+
+lemma set_ltree_addr_op_impl (address : adrs, ltree_addr : int):
+    hoare[M.__set_ltree_addr :
+        arg = (address, W32.of_int ltree_addr) ==> res = set_ltree_addr address ltree_addr].
+proof. proc. auto. qed.
+
+lemma set_tree_height_op_impl (address : adrs, tree_height : int):
+    tree_height_pre tree_height =>
+        hoare[M.__set_tree_height :
+            arg = (address, W32.of_int tree_height) ==> res = set_tree_height address tree_height].
+proof. move => pre_cond. proc. auto. qed.
+
+lemma get_set_tree_height (address : adrs, tree_height : int) :
+    tree_height_pre tree_height => 
+    get_tree_height (set_tree_height address tree_height) = tree_height.
+proof.
+rewrite /get_tree_height /set_tree_height.
+progress.
+apply word_int.
+smt().
+qed.
+
+lemma set_tree_index_op_impl (address : adrs, tree_index) : 
+    hoare[M.__set_tree_index :
+        arg = (address, W32.of_int tree_index) ==> res = set_tree_index address tree_index].
+proof. proc. auto. qed.
+
+lemma get_set_tree_index (address : adrs, tree_index : int) :
+  0 <= tree_index < W32.modulus => (* i.e. tree_index fits in a u32 *)
+  get_tree_index (set_tree_index address tree_index) = tree_index.  
+proof.
+rewrite /get_tree_index /set_tree_index.
+progress.
+apply word_int.
+ smt().
+qed.
+
+lemma set_key_and_mask_op_impl (address : adrs, key_and_mask : int):
+    hoare[M.__set_key_and_mask :
+        arg = (address, W32.of_int key_and_mask) ==> res = set_key_and_mask address key_and_mask].
+proof. proc. auto. qed.
+
+op zero_addr : adrs = Array8.init (fun _ => W32.zero). 
+lemma zero_addr_op_impl (address : adrs) :
+    hoare[M._zero_address : true ==> res = zero_addr].
+proof.
+proc.
+while (0 <= i <= 8 /\ 
+      (forall (k : int), 0 <= k < i => (addr.[k] = W32.zero))); auto => /> ; smt(get_setE tP initiE).
+qed.
 
 (******************************************************************************)
 
